src/program_proof/tulip/program/replica/replica.v
@@ -1,4 +1,5 @@
-From Perennial.program_proof.tulip.invariance Require Import validate execute accept learn.
+From Perennial.program_proof.tulip.invariance Require Import
+  validate execute accept learn local_read.
 From Perennial.program_proof Require Import std_proof.
 From Perennial.program_proof.tulip.program Require Import prelude.
 From Perennial.program_proof.tulip.program.replica Require Import
@@ -49,19 +50,214 @@ Section replica.
       "#HtxnlogP" ∷ readonly (rp ↦[Replica :: "txnlog"] #txnlog) ∗
       "#Htxnlog"  ∷ is_txnlog txnlog gid γ.
 
-  Definition is_replica_idx (rp : loc) α : iProp Σ :=
+  Definition is_replica_idx (rp : loc) γ α : iProp Σ :=
     ∃ (idx : loc),
       "#HidxP" ∷ readonly (rp ↦[Replica :: "idx"] #idx) ∗
-      "#Hidx"  ∷ is_index idx α.
+      "#Hidx"  ∷ is_index idx γ α.
 
-  Definition is_replica (rp : loc) : iProp Σ :=
-    ∃ (mu : loc) (gid rid : u64) γ α,
+  Definition is_replica (rp : loc) gid rid γ : iProp Σ :=
+    ∃ (mu : loc) α,
       "#HmuP"    ∷ readonly (rp ↦[Replica :: "mu"] #mu) ∗
       "#Hlock"   ∷ is_lock tulipNS #mu (own_replica rp gid rid γ α) ∗
       "#Htxnlog" ∷ is_replica_txnlog rp gid γ ∗
-      "#Hidx"    ∷ is_replica_idx rp α ∗
+      "#Hidx"    ∷ is_replica_idx rp γ α ∗
       "#Hinv"    ∷ know_tulip_inv γ ∗
-      "%Hgid"    ∷ ⌜gid ∈ gids_all⌝.
+      "%Hgid"    ∷ ⌜gid ∈ gids_all⌝ ∗
+      "%Hrid"    ∷ ⌜rid ∈ rids_all⌝.
+
+  Theorem wp_Replica__logRead (rp : loc) (ts : u64) (key : string) :
+    {{{ True }}}
+      Replica__logRead #rp #ts #(LitString key)
+    {{{ RET #(); True }}}.
+  Proof.
+    (*@ func (rp *Replica) logRead(ts uint64, key string) {                     @*)
+    (*@     // TODO: Create an inconsistent log entry for reading @key at @ts.  @*)
+    (*@ }                                                                       @*)
+  Admitted.
+
+  Theorem wp_Replica__Read (rp : loc) (tsW : u64) (key : string) gid rid γ :
+    let ts := uint.nat tsW in
+    ts ≠ O ->
+    key ∈ keys_all ->
+    key_to_group key = gid ->
+    is_replica rp gid rid γ -∗
+    {{{ True }}}
+      Replica__Read #rp #tsW #(LitString key)
+    {{{ (t : u64) (v : dbval) (ok : bool), RET (#t, dbval_to_val v, #ok);
+        if ok
+        then if decide (uint.nat t = O)
+             then is_repl_hist_at γ key (pred ts) v
+             else is_repl_hist_at γ key (uint.nat t) v ∗
+                  read_promise γ gid rid key (uint.nat t) ts ∗
+                  ⌜(uint.nat t < pred ts)⌝
+        else True
+    }}}.
+  Proof.
+    iIntros (ts Htsnz Hkey Hkg) "#Hrp".
+    iIntros (Φ) "!> _ HΦ".
+    wp_rec.
+
+    (*@ func (rp *Replica) Read(ts uint64, key string) (uint64, tulip.Value, bool) { @*)
+    (*@     tpl := rp.idx.GetTuple(key)                                         @*)
+    (*@                                                                         @*)
+    iNamed "Hrp". iNamed "Hidx".
+    wp_loadField.
+    wp_apply (wp_Index__GetTuple with "Hidx"); first apply Hkey.
+    iIntros (tpl) "#Htpl".
+
+    (*@     t1, v1 := tpl.ReadVersion(ts)                                       @*)
+    (*@                                                                         @*)
+    wp_apply (wp_Tuple__ReadVersion_xphys with "Htpl").
+    iIntros (t1 v1) "Hread1".
+    wp_pures.
+
+    (*@     if t1 == 0 {                                                        @*)
+    (*@         // Fast-path read.                                              @*)
+    (*@         return 0, v1, true                                              @*)
+    (*@     }                                                                   @*)
+    (*@                                                                         @*)
+    case_bool_decide as Ht1; wp_pures.
+    { iApply "HΦ". by case_decide; last inv Ht1. }
+
+    (*@     rp.mu.Lock()                                                        @*)
+    (*@                                                                         @*)
+    wp_loadField.
+    wp_apply (wp_Mutex__Lock with "Hlock").
+    iIntros "[Hlocked Hrp]".
+
+    (*@     ok := rp.readableKey(ts, key)                                       @*)
+    (*@                                                                         @*)
+    do 2 iNamed "Hrp".
+    wp_apply (wp_Replica__readableKey with "Hptsmsptsm"); first apply Hkey.
+    iIntros (ok) "[Hptsmsptsm %Hreadable]".
+    wp_pures.
+
+    (*@     if !ok {                                                            @*)
+    (*@         // Trying to read a tuple that is locked by a lower-timestamp   @*)
+    (*@         // transaction. This read has to fail because the value to be read is @*)
+    (*@         // undetermined---the prepared transaction might or might not commit. @*)
+    (*@         rp.mu.Unlock()                                                  @*)
+    (*@         return 0, tulip.Value{}, false                                  @*)
+    (*@     }                                                                   @*)
+    (*@                                                                         @*)
+    destruct ok; wp_pures; last first.
+    { wp_loadField.
+      wp_apply (wp_Mutex__Unlock with "[-HΦ]").
+      { by iFrame "Hlock Hlocked ∗ # %". }
+      wp_pures.
+      by iApply ("HΦ" $! _ None).
+    }
+
+    (*@     t2, v2 := tpl.ReadVersion(ts)                                       @*)
+    (*@                                                                         @*)
+    assert (is_Some (histm !! key)) as [hist Hhist].
+    { unshelve epose proof (execute_cmds_apply_cmds cloga ilog cm histm _) as Happly.
+      { by eauto 10. }
+      pose proof (apply_cmds_dom _ _ _ Happly) as Hdomhistm.
+      by rewrite -elem_of_dom Hdomhistm.
+    }
+    iDestruct (big_sepM_lookup_acc with "Hhistm") as "[Hhist HhistmC]"; first apply Hhist.
+    wp_apply (wp_Tuple__ReadVersion with "Htpl Hhist").
+    iIntros (t2 v2) "[Hhist #Hlb]".
+    iDestruct ("HhistmC" with "Hhist") as "Hhistm".
+    wp_pures.
+
+    (*@     if t2 == 0 {                                                        @*)
+    (*@         // Fast-path read.                                              @*)
+    (*@         rp.mu.Unlock()                                                  @*)
+    (*@         return 0, v2, true                                              @*)
+    (*@     }                                                                   @*)
+    (*@                                                                         @*)
+    case_bool_decide as Ht2; wp_pures.
+    { wp_loadField.
+      wp_apply (wp_Mutex__Unlock with "[-HΦ]").
+      { by iFrame "Hlock Hlocked ∗ # %". }
+      wp_pures.
+      iApply "HΦ".
+      by case_decide; last inv Ht2.
+    }
+
+    (*@     // Slow-path read.                                                  @*)
+    (*@     rp.bumpKey(ts, key)                                                 @*)
+    (*@                                                                         @*)
+    wp_apply (wp_Replica__bumpKey with "Hptsmsptsm").
+    { clear -Htsnz. word. }
+    { apply Hkey. }
+    iIntros (spts) "[Hptsmsptsm %Hspts]".
+
+    (*@     // TODO: An optimization is to create a log entry iff the smallest  @*)
+    (*@     // preparable timestamp is actually bumped, which can be checked with the @*)
+    (*@     // return value of @rp.bumpKey.                                     @*)
+    (*@                                                                         @*)
+    (*@     // Logical actions: Execute() and then LocalRead(@ts, @key)         @*)
+    (*@     rp.logRead(ts, key)                                                 @*)
+    (*@                                                                         @*)
+    wp_pures.
+    wp_apply wp_Replica__logRead.
+    iApply fupd_wp.
+    iInv "Hinv" as "> HinvO" "HinvC".
+    iNamed "HinvO".
+    iDestruct (big_sepS_elem_of_acc with "Hgroups") as "[Hgroup HgroupsC]"; first apply Hgid.
+    iDestruct (big_sepS_elem_of_acc with "Hrgs") as "[Hrg HrgsC]"; first apply Hgid.
+    iDestruct (big_sepS_elem_of_acc with "Hrg") as "[Hrp HrgC]"; first apply Hrid.
+    (* First catching up the consistent log. *)
+    destruct Hcloga as [cmdsa ->].
+    iMod (replica_inv_execute with "Hclogalb Hclog Hilog Hgroup Hrp")
+      as "(Hclog & Hilog & Hgroup & Hrp)".
+    iMod (replica_inv_local_read key ts with "Hclog Hilog Hgroup Hrp")
+      as "(Hclog & Hilog & Hgroup & Hrp & #Hpromise & #Hrepllb)".
+    { apply Hkey. }
+    { apply Hkg. }
+    { apply Hexec. }
+    { simpl.
+      rewrite /key_readable in Hreadable.
+      destruct (ptsm !! key) as [pts |] eqn:Hpts; rewrite Hpts in Hreadable; last done.
+      exists spts, pts.
+      do 3 (split; first done).
+      clear -Hreadable. word.
+    }
+    iDestruct ("HgroupsC" with "Hgroup") as "Hgroups".
+    iDestruct ("HrgC" with "Hrp") as "Hrg".
+    iDestruct ("HrgsC" with "Hrg") as "Hrgs".
+    iMod ("HinvC" with "[$Htxnsys $Hkeys $Hgroups $Hrgs]") as "_".
+    iModIntro.
+
+    (*@     rp.mu.Unlock()                                                      @*)
+    (*@     return t2, v2, true                                                 @*)
+    (*@ }                                                                       @*)
+    wp_loadField.
+    wp_apply (wp_Mutex__Unlock with "[-HΦ]").
+    { iFrame "Hlock Hlocked ∗ # %".
+      iPureIntro. simpl.
+      exists ptgsm.
+      split; first done.
+      split.
+      { rewrite Forall_forall.
+        intros [n c] Hilog. simpl.
+        apply elem_of_app in Hilog as [Hilog | Hnewc].
+        { rewrite Forall_forall in Hvicmds. by specialize (Hvicmds _ Hilog). }
+        rewrite elem_of_list_singleton in Hnewc.
+        by inv Hnewc.
+      }
+      { rewrite merge_clog_ilog_snoc_ilog; last done.
+        rewrite /execute_cmds foldl_snoc execute_cmds_unfold Hexec /=.
+        erewrite lookup_alter_Some; last apply Hspts.
+        f_equal.
+      }
+    }
+    wp_pures.
+    iApply "HΦ".
+    case_decide as Hnz; first done.
+    iDestruct "Hlb" as "[Hlb' %Hv2]".
+    clear Ht2.
+    destruct Hv2 as (Hv2 & Ht2 & Hlenhist).
+    rewrite Ht2.
+    iFrame "Hrepllb Hpromise".
+    iPureIntro.
+    split.
+    { by rewrite -last_lookup. }
+    { clear -Ht2 Hnz Hlenhist. word. }
+  Qed.
 
   Theorem wp_Replica__multiwrite rp (tsW : u64) pwrsS pwrsL pwrs histm gid γ α :
     let ts := uint.nat tsW in
@@ -70,7 +266,7 @@ Section replica.
     dom histm = keys_all ->
     safe_extension ts pwrs histm ->
     ([∗ map] k ↦ h ∈ filter_group gid histm', is_repl_hist_lb γ k h) -∗
-    is_replica_idx rp α -∗
+    is_replica_idx rp γ α -∗
     {{{ own_dbmap_in_slice pwrsS pwrsL pwrs ∗ own_replica_histm rp histm α }}}
       Replica__multiwrite #rp #tsW (to_val pwrsS)
     {{{ RET #(); 
@@ -298,7 +494,7 @@ Section replica.
     valid_pwrs gid pwrs ->
     group_histm_lbs_from_log γ gid cloga' -∗
     is_txn_log_lb γ gid cloga' -∗
-    is_replica_idx rp α -∗
+    is_replica_idx rp γ α -∗
     {{{ own_dbmap_in_slice pwrsS pwrsL pwrs ∗
         own_replica_with_cloga_no_lsna rp cloga gid rid γ α
     }}}
@@ -617,7 +813,7 @@ Section replica.
     valid_ccommand gid cmd ->
     group_histm_lbs_from_log γ gid cloga' -∗
     is_txn_log_lb γ gid cloga' -∗
-    is_replica_idx rp α -∗
+    is_replica_idx rp γ α -∗
     {{{ own_pwrs_slice pwrsS cmd ∗
         own_replica_with_cloga_no_lsna rp cloga gid rid γ α
     }}}
@@ -670,8 +866,8 @@ Section replica.
     }
   Qed.
 
-  Theorem wp_Replica__Start rp :
-    is_replica rp -∗
+  Theorem wp_Replica__Start rp gid rid γ :
+    is_replica rp gid rid γ -∗
     {{{ True }}}
       Replica__Start #rp
     {{{ RET #(); True }}}.
