src/program_proof/tulip/program/tuple/tuple.v
@@ -11,12 +11,12 @@ End res.
 Section program.
   Context `{!heapGS Σ, !tulip_ghostG Σ}.
 
-  Definition is_tuple (tuple : loc) (key : string) (α : replica_names) : iProp Σ.
+  Definition is_tuple (tuple : loc) (key : string) (γ : tulip_names) (α : replica_names) : iProp Σ.
   Admitted.
 
   #[global]
-  Instance is_tuple_persistent tuple key α :
-    Persistent (is_tuple tuple key α).
+  Instance is_tuple_persistent tuple key γ α :
+    Persistent (is_tuple tuple key γ α).
   Admitted.
 
   Theorem wp_Tuple__AppendVersion (tuple : loc) (tsW : u64) (value : string) key hist γ α :
@@ -24,7 +24,7 @@ Section program.
     let hist' := last_extend ts hist ++ [Some value] in
     (length hist ≤ ts)%nat ->
     is_repl_hist_lb γ key hist' -∗
-    is_tuple tuple key α -∗
+    is_tuple tuple key γ α -∗
     {{{ own_phys_hist_half α key hist }}}
       Tuple__AppendVersion #tuple #tsW #(LitString value)
     {{{ RET #(); own_phys_hist_half α key hist' }}}.
@@ -36,20 +36,38 @@ Section program.
     let hist' := last_extend ts hist ++ [None] in
     (length hist ≤ ts)%nat ->
     is_repl_hist_lb γ key hist' -∗
-    is_tuple tuple key α -∗
+    is_tuple tuple key γ α -∗
     {{{ own_phys_hist_half α key hist }}}
       Tuple__KillVersion #tuple #tsW
     {{{ RET #(); own_phys_hist_half α key hist' }}}.
   Proof.
   Admitted.
 
-  (* TODO *)
-  Theorem wp_Tuple__ReadVersion (tuple : loc) (tsW : u64) key α :
+  Theorem wp_Tuple__ReadVersion_xphys (tuple : loc) (tsW : u64) key γ α :
     let ts := uint.nat tsW in
-    is_tuple tuple key α -∗
+    is_tuple tuple key γ α -∗
     {{{ True }}}
       Tuple__ReadVersion #tuple #tsW
-    {{{ (v : dbval) (ok : bool), RET (dbval_to_val v, #ok); True }}}.
+    {{{ (t : u64) (v : dbval), RET (#t, dbval_to_val v);
+        if decide (uint.nat t = O) then is_repl_hist_at γ key (pred ts) v else True
+    }}}.
+  Proof.
+  Admitted.
+
+  Theorem wp_Tuple__ReadVersion (tuple : loc) (tsW : u64) key hist γ α :
+    let ts := uint.nat tsW in
+    is_tuple tuple key γ α -∗
+    {{{ own_phys_hist_half α key hist }}}
+      Tuple__ReadVersion #tuple #tsW
+    {{{ (t : u64) (v : dbval), RET (#t, dbval_to_val v);
+        own_phys_hist_half α key hist ∗
+        if decide (uint.nat t = O)
+        then is_repl_hist_at γ key (pred ts) v
+        else is_repl_hist_lb γ key hist ∗
+             ⌜last hist = Some v⌝ ∗
+             ⌜uint.nat t = pred (length hist)⌝ ∗
+             ⌜(length hist < ts)%nat⌝
+    }}}.
   Proof.
   Admitted.
 
